src/MatMul.fst
@@ -5,8 +5,18 @@ open Vector
 open MatrixType
 open Matrix
 
+
+let triangular_compat (#n: pos) (m1 m2: mat n) : prop =
+  (lower m1 /\ lower m2) \/ (upper m1 /\ upper m2)
+
 (* matrix-matrix multiplication via block formula *)
-let rec mat_mul (#n: pos) (m1 m2: mat n) : mat n =
+let rec mat_mul (#n: pos) (m1 m2: mat n) : r: mat n
+  {(lower m1 /\ lower m2 ==> lower r) /\
+    (upper m1 /\ upper m2 ==> upper r) /\
+    (triangular_compat m1 m2 /\ unit_diag m1 /\ unit_diag m2 ==> unit_diag r) /\
+    (triangular_compat m1 m2 /\ pos_diag m1 /\ pos_diag m2 ==> pos_diag r) /\
+    (triangular_compat m1 m2 /\ nnz_diag m1 /\ nnz_diag m2 ==> nnz_diag r) /\
+    (is_id m1 ==> r == m2) /\ (is_id m2 ==> r == m1)} =
   match m1 with
   | Mat1 a -> let Mat1 b = m2 in Mat1 (scalar_mul a b)
   | MatN m1' c1 a1 b1 ->
@@ -15,72 +25,7 @@ let rec mat_mul (#n: pos) (m1 m2: mat n) : mat n =
       (vec_add (vec_scalar_mul c1 a2) (mat_vec_mul m1' c2))
       (scalar_add (scalar_mul a1 a2) (inner_prod b1 c2))
       (vec_add (vec_scalar_mul b2 a1) (vec_mat_mul b1 m2'))
-
-let triangular_compat (#n: pos) (m1 m2: mat n) : prop =
-  (lower m1 /\ lower m2) \/ (upper m1 /\ upper m2)
-
-let rec mat_mul_lower (#n: pos) (m1 m2: mat n)
-    : Lemma (requires lower m1 /\ lower m2)
-      (ensures lower (mat_mul m1 m2))
-      [SMTPat (lower (mat_mul m1 m2))] =
-  match m1 with
-  | Mat1 _ -> let Mat1 _ = m2 in ()
-  | MatN m1' _ _ _ ->
-    let MatN m2' _ _ _ = m2 in
-    mat_mul_lower m1' m2'
-
-let rec mat_mul_upper (#n: pos) (m1 m2: mat n)
-    : Lemma (requires upper m1 /\ upper m2)
-      (ensures upper (mat_mul m1 m2))
-      [SMTPat (upper (mat_mul m1 m2))] =
-  match m1 with
-  | Mat1 _ -> let Mat1 _ = m2 in ()
-  | MatN m1' _ _ _ ->
-    let MatN m2' _ _ _ = m2 in
-    mat_mul_upper m1' m2'
-
-let rec mat_mul_unit_diag (#n: pos) (m1 m2: mat n)
-    : Lemma (requires triangular_compat m1 m2 /\ unit_diag m1 /\ unit_diag m2)
-      (ensures unit_diag (mat_mul m1 m2))
-      [SMTPat (unit_diag (mat_mul m1 m2))] =
-  match m1 with
-  | Mat1 _ -> let Mat1 _ = m2 in ()
-  | MatN m1' _ _ _ ->
-    let MatN m2' _ _ _ = m2 in
-    mat_mul_unit_diag m1' m2'
-
-let rec mat_mul_pos_diag (#n: pos) (m1 m2: mat n)
-    : Lemma (requires triangular_compat m1 m2 /\ pos_diag m1 /\ pos_diag m2)
-      (ensures pos_diag (mat_mul m1 m2))
-      [SMTPat (pos_diag (mat_mul m1 m2))] =
-  match m1 with
-  | Mat1 _ -> let Mat1 _ = m2 in ()
-  | MatN m1' _ _ _ ->
-    let MatN m2' _ _ _ = m2 in
-    mat_mul_pos_diag m1' m2'
-
-let rec mat_mul_nnz_diag (#n: pos) (m1 m2: mat n)
-    : Lemma (requires triangular_compat m1 m2 /\ nnz_diag m1 /\ nnz_diag m2)
-      (ensures nnz_diag (mat_mul m1 m2))
-      [SMTPat (nnz_diag (mat_mul m1 m2))] =
-  match m1 with
-  | Mat1 _ -> let Mat1 _ = m2 in ()
-  | MatN m1' _ _ _ ->
-    let MatN m2' _ _ _ = m2 in
-    mat_mul_nnz_diag m1' m2'
-
-let rec mat_mul_id_l (#n: pos) (m: mat n)
-    : Lemma (mat_mul id_mat m == m) [SMTPat (mat_mul id_mat m)] =
-  match m with
-  | Mat1 _ -> ()
-  | MatN m' _ _ _ -> mat_mul_id_l m'
-
-let rec mat_mul_id_r (#n: pos) (m: mat n)
-    : Lemma (mat_mul m id_mat == m) [SMTPat (mat_mul m id_mat)] =
-  match m with
-  | Mat1 _ -> ()
-  | MatN m' _ _ _ -> mat_mul_id_r m'
-
+      
 (* mul associates with mat-vec mul *)
 assume val mat_vec_mul_assoc (#n: pos) (m1 m2: mat n) (c: cvec n)
     : Lemma (mat_vec_mul (mat_mul m1 m2) c == mat_vec_mul m1 (mat_vec_mul m2 c))
@@ -93,11 +38,7 @@ assume val mat_mul_perm (#n: pos) (m1 m2: mat n)
     : Lemma (requires perm m1 /\ perm m2)
       (ensures perm (mat_mul m1 m2))
       [SMTPat (perm (mat_mul m1 m2))]
-
-assume val mat_mul_assoc (#n: pos) (m1 m2 m3: mat n)
-    : Lemma (mat_mul (mat_mul m1 m2) m3 == mat_mul m1 (mat_mul m2 m3))
-      [SMTPat (mat_mul (mat_mul m1 (transpose m2)) m3)]
-
+      
 assume val mat_mul_sub_distr (#n: pos) (m m1 m2: mat n)
     : Lemma (mat_mul m (mat_sub m1 m2) == mat_sub (mat_mul m m1) (mat_mul m m2))
       [SMTPat (mat_mul m (mat_sub m1 m2))]
@@ -108,9 +49,11 @@ assume val mat_mul_outer_prod (#n: pos) (m: mat n) (c: cvec n) (r: rvec n)
 
 assume val transpose_perm (#n: pos) (m: mat n)
     : Lemma (requires perm m)
-      (ensures perm (transpose m) /\ is_inverse m (transpose m))
+      (ensures perm (transpose m) /\ 
+        mat_mul m (transpose m) == id_mat /\
+        mat_mul (transpose m) m == id_mat)
+      [SMTPat (perm m)]
 
-assume val perm_inv_l (#n: pos) (p: mat n) (m: mat n)
-    : Lemma (requires perm p)
-      (ensures mat_mul (transpose p) (mat_mul p m) == m)
-      [SMTPat (mat_mul (transpose p) (mat_mul p m))]
+assume val mat_mul_assoc_transp (#n: pos) (m1 m2 m3: mat n)
+    : Lemma (mat_mul (mat_mul m1 (transpose m2)) m3 == mat_mul m1 (mat_mul (transpose m2) m3))
+      [SMTPat (mat_mul (mat_mul m1 (transpose m2)) m3)]
