src/MatrixType.fst
@@ -19,9 +19,6 @@ let rec upper (#n: pos) (m: mat n) : prop =
   | Mat1 _ -> True
   | MatN m' col _ _ -> upper m' /\ is_zero_vec col
 
-assume val one_by_one_lower : m:mat 1 -> Lemma (lower m) [SMTPat (lower m)]
-assume val one_by_one_upper : m:mat 1 -> Lemma (upper m) [SMTPat (upper m)]
-
 let diagonal (#n: pos) (m: mat n) : prop = lower m /\ upper m
 
 (* what's on the diagonal *)
@@ -62,14 +59,14 @@ assume val spd_pos_diag (#n: pos) (m: mat n) : Lemma (requires spd m) (ensures p
 assume val rowsdd_nnz_diag (#n: pos) (m: mat n)
     : Lemma (requires rowsdd m) (ensures nnz_diag m) [SMTPat (rowsdd m)]
 
-assume val destruct_rowsdd (#n: pos{n >= 2}) (m: mat n) :
-    Lemma (requires rowsdd m) (ensures (let MatN m' b a c = m in rowsdd m' /\ is_nnz a)) [SMTPat (rowsdd m)]
+assume val destruct_rowsdd (#n: pos{n >= 2}) (m: mat n)
+    : Lemma (requires rowsdd m) (ensures (let MatN m' _ a _ = m in rowsdd m' /\ is_nnz a)) [SMTPat (rowsdd m)]
 
-assume val destruct_spd (#n: pos{n >= 2}) (m: mat n) :
-    Lemma (requires spd m) (ensures (let MatN m' b a c = m in spd m' /\ is_pos a)) [SMTPat (spd m)]
+assume val destruct_spd (#n: pos{n >= 2}) (m: mat n)
+    : Lemma (requires spd m) (ensures (let MatN m' _ a _ = m in spd m' /\ is_pos a)) [SMTPat (spd m)]
 
-assume val inv_1x1_nnz_diag (m:mat 1) :
-  Lemma (requires inv m) (ensures nnz_diag m) [SMTPat (inv (m <: mat 1))]
+assume val inv_1x1_nnz_diag (m: mat 1)
+    : Lemma (requires inv m) (ensures nnz_diag m) [SMTPat (inv (m <: mat 1))]
 
 (* shorthands *)
 let unit_lower (#n: pos) (m: mat n) : prop = lower m /\ unit_diag m
@@ -88,11 +85,11 @@ let rec zero_mat (#n: pos) : mat n =
 
 let is_zero_mat (#n: pos) (m: mat n) : prop = m == zero_mat
 
-// let rec id_mat_diagonal (#n: pos) : Lemma (diagonal (id_mat #n)) [SMTPat (id_mat #n)] =
-//   if n = 1 then () else id_mat_diagonal #(n - 1)
+let rec id_mat_diagonal (#n: pos) : Lemma (diagonal (id_mat #n)) [SMTPat (id_mat #n)] =
+  if n = 1 then () else id_mat_diagonal #(n - 1)
 
-// let rec id_mat_unit_diag (#n: pos) : Lemma (unit_diag (id_mat #n)) [SMTPat (id_mat #n)] =
-//   if n = 1 then () else id_mat_unit_diag #(n - 1)
+let rec id_mat_unit_diag (#n: pos) : Lemma (unit_diag (id_mat #n)) [SMTPat (id_mat #n)] =
+  if n = 1 then () else id_mat_unit_diag #(n - 1)
 
 (* permutation matrix *)
 assume val perm: #n: pos -> mat n -> prop
@@ -101,8 +98,8 @@ assume val perm_is_inv (#n: pos) (m: mat n) : Lemma (requires perm m) (ensures i
 
 assume val id_mat_is_perm (#n: pos) : Lemma (perm (id_mat #n)) [SMTPat (id_mat #n)]
 
-assume val augment_perm (#n: pos) (m: mat n{perm m}) :
-  Lemma (perm (MatN m zero_vec one zero_vec)) [SMTPat (perm m)]
+assume val augment_perm (#n: pos) (m: mat n) :
+  Lemma (requires perm m) (ensures perm (MatN m zero_cvec one zero_rvec)) [SMTPat (perm m)]
 
 (* top-left entry is nonzero *)
 let top_left_nnz (#n: pos) (m: mat n) : prop =
