src/Vector.fst
@@ -5,6 +5,7 @@ open Scalar
 type orient = | Row | Col
 let flip (o: orient) : orient = match o with | Row -> Col | Col -> Row
 
+// or: size function computes size of vector. use as a refinement
 noeq type vec : orient -> pos -> Type =
   | Vec1 : #o: orient -> num -> vec o 1
   | VecN : #o: orient -> #n: pos -> vec o n -> num -> vec o (n + 1)
@@ -25,34 +26,18 @@ let zero_cvec (#n: pos) : cvec n = zero_vec #Col #n
 let is_zero_vec (#o: orient) (#n: pos) (v: vec o n) : prop = v == zero_vec #o #n
 
 (* add vectors *)
-let rec vec_add (#o: orient) (#n: pos) (v1 v2: vec o n) : vec o n =
+let rec vec_add (#o: orient) (#n: pos) (v1 v2: vec o n) : r: vec o n 
+  {(is_zero_vec v1 ==> r == v2) /\ (is_zero_vec v2 ==> r == v1)} =
   match v1 with
   | Vec1 x -> let Vec1 y = v2 in Vec1 (scalar_add x y)
   | VecN v1' x -> let VecN v2' y = v2 in VecN (vec_add v1' v2') (scalar_add x y)
 
-let rec vec_add_zero_l (#o: orient) (#n: pos) (v1 v2: vec o n)
-    : Lemma (requires is_zero_vec v1) (ensures vec_add v1 v2 == v2) [SMTPat (vec_add v1 v2)] =
-  match v1 with 
-  | Vec1 _ -> let Vec1 _ = v2 in ()
-  | VecN v1' _ -> let VecN v2' _ = v2 in vec_add_zero_l v1' v2'
-
-let rec vec_add_zero_r (#o: orient) (#n: pos) (v1 v2: vec o n)
-    : Lemma (requires is_zero_vec v2) (ensures vec_add v1 v2 == v1) [SMTPat (vec_add v1 v2)] =
-  match v2 with
-  | Vec1 _ -> let Vec1 _ = v1 in ()
-  | VecN v2' _ -> let VecN v1' _ = v1 in vec_add_zero_r v1' v2'
-
 (* negate a vector *)
-let rec vec_neg (#o: orient) (#n: pos) (v: vec o n) : vec o n =
+let rec vec_neg (#o: orient) (#n: pos) (v: vec o n) : r: vec o n 
+  {is_zero_vec v ==> is_zero_vec r} =
   match v with
   | Vec1 x -> Vec1 (scalar_neg x)
   | VecN v' x -> VecN (vec_neg v') (scalar_neg x)
-
-let rec vec_neg_zero (#o: orient) (#n: pos) (v: vec o n)
-    : Lemma (requires is_zero_vec v) (ensures is_zero_vec (vec_neg v)) [SMTPat (vec_neg v)] =
-  match v with
-  | Vec1 _ -> ()
-  | VecN v' _ -> vec_neg_zero v'
 
 let rec vec_neg_add_inv_l (#o: orient) (#n: pos) (v: vec o n)
     : Lemma (is_zero_vec (vec_add v (vec_neg v))) [SMTPat (vec_add v (vec_neg v))] =
@@ -73,35 +58,22 @@ let rec vec_neg_involutive (#o: orient) (#n: pos) (v: vec o n)
   | VecN v' _ -> vec_neg_involutive v'
 
 (* vector-scalar mul *)
-let rec vec_scalar_mul (#o: orient) (#n: pos) (v: vec o n) (a: num) : vec o n =
+let rec vec_scalar_mul (#o: orient) (#n: pos) (v: vec o n) (a: num) : r: vec o n
+  {(is_one a ==> r == v) /\ (is_zero_vec v ==> is_zero_vec r) /\ (is_zero a ==> is_zero_vec r)} =
   match v with
   | Vec1 x -> Vec1 (scalar_mul x a)
   | VecN v' x -> VecN (vec_scalar_mul v' a) (scalar_mul x a)
 
-let rec vec_scalar_mul_one (#o: orient) (#n: pos) (v: vec o n) (a: num)
-    : Lemma (requires is_one a) (ensures vec_scalar_mul v a == v) [SMTPat (vec_scalar_mul v a)] =
+let rec vec_scalar_mul_neg (#o: orient) (#n: pos) (v: vec o n) (a: num)
+    : Lemma (vec_scalar_mul v (scalar_neg a) == vec_neg (vec_scalar_mul v a))
+      [SMTPat (vec_scalar_mul v (scalar_neg a))] =
   match v with
   | Vec1 _ -> ()
-  | VecN v' _ -> vec_scalar_mul_one v' a
-
-let rec vec_scalar_mul_zero (#o: orient) (#n: pos) (v: vec o n) (a: num)
-    : Lemma (requires is_zero_vec v)
-      (ensures is_zero_vec (vec_scalar_mul v a))
-      [SMTPat (vec_scalar_mul v a)] =
-  match v with
-  | Vec1 _ -> ()
-  | VecN v' _ -> vec_scalar_mul_zero v' a
-
-let rec vec_scalar_mul_zero_scalar (#o: orient) (#n: pos) (v: vec o n) (a: num)
-    : Lemma (requires is_zero a)
-      (ensures is_zero_vec (vec_scalar_mul v a))
-      [SMTPat (vec_scalar_mul v a)] =
-  match v with
-  | Vec1 _ -> ()
-  | VecN v' _ -> vec_scalar_mul_zero_scalar v' a
+  | VecN v' _ -> vec_scalar_mul_neg v' a
 
 (* vector-scalar div *)
-let rec vec_scalar_div (#o: orient) (#n: pos) (v: vec o n) (a: num{is_nnz a}) : vec o n =
+let rec vec_scalar_div (#o: orient) (#n: pos) (v: vec o n) (a: num{is_nnz a}) : r: vec o n 
+  {vec_scalar_mul r a == v} =
   match v with
   | Vec1 x -> Vec1 (scalar_div x a)
   | VecN v' x -> VecN (vec_scalar_div v' a) (scalar_div x a)
@@ -114,37 +86,19 @@ let rec vec_scalar_div_assoc (#o: orient) (#n: pos) (v: vec o n)
   | Vec1 _ -> ()
   | VecN v' _ -> vec_scalar_div_assoc v' a1 a2
 
-let rec vec_scalar_div_mul (#o: orient) (#n: pos) (v: vec o n) (a: num{is_nnz a})
-    : Lemma (vec_scalar_mul (vec_scalar_div v a) a == v)
-      [SMTPat (vec_scalar_mul (vec_scalar_div v a) a)] =
-  match v with
-  | Vec1 _ -> ()
-  | VecN v' _ -> vec_scalar_div_mul v' a
-
 (* inner product *)
-let rec inner_prod (#n: pos) (r: rvec n) (c: cvec n) : num =
+let rec inner_prod (#n: pos) (r: rvec n) (c: cvec n) : a: num 
+  {(is_zero_vec r \/ is_zero_vec c) ==> is_zero a} =
   match r with
   | Vec1 x -> let Vec1 y = c in scalar_mul x y
   | VecN r' rx -> let VecN c' cy = c in scalar_add (inner_prod r' c') (scalar_mul rx cy)
 
-let rec inner_prod_zero (#n: pos) (r: rvec n) (c: cvec n)
-    : Lemma (requires is_zero_vec r \/ is_zero_vec c) (ensures is_zero (inner_prod r c))
-      [SMTPat (inner_prod r c)] =
-  match r with
-  | Vec1 _ -> let Vec1 _ = c in ()
-  | VecN r' _ -> let VecN c' _ = c in inner_prod_zero r' c'
-
 (* transpose vector *)
-let rec vec_trans (#o: orient) (#n: pos) (v: vec o n) : vec (flip o) n =
+let rec vec_trans (#o: orient) (#n: pos) (v: vec o n) : r: vec (flip o) n 
+  {is_zero_vec v ==> is_zero_vec r} =
   match v with
   | Vec1 x -> Vec1 x
   | VecN v' x -> VecN (vec_trans v') x
-
-let rec vec_trans_zero (#o: orient) (#n: pos) (v: vec o n)
-    : Lemma (requires is_zero_vec v) (ensures is_zero_vec (vec_trans v)) [SMTPat (vec_trans v)] =
-  match v with
-  | Vec1 _ -> ()
-  | VecN v' _ -> vec_trans_zero v'
 
 let rec vec_trans_scalar_div (#o: orient) (#n: pos) (v: vec o n) (a: num{is_nnz a})
     : Lemma (vec_trans (vec_scalar_div v a) == vec_scalar_div (vec_trans v) a)
@@ -158,3 +112,46 @@ let rec vec_trans_involutive (#o: orient) (#n: pos) (v: vec o n)
   match v with
   | Vec1 _ -> ()
   | VecN v' _ -> vec_trans_involutive v'
+
+let rec vec_neg_add_dist (#o: orient) (#n: pos) (v1 v2: vec o n)
+    : Lemma (vec_neg (vec_add v1 v2) == vec_add (vec_neg v1) (vec_neg v2))
+      [SMTPat (vec_neg (vec_add v1 v2))] =
+  match v1 with
+  | Vec1 _ -> let Vec1 _ = v2 in ()
+  | VecN v1' _ -> let VecN v2' _ = v2 in vec_neg_add_dist v1' v2'
+
+let rec inner_prod_neg_r (#n: pos) (r: rvec n) (c: cvec n)
+    : Lemma (inner_prod r (vec_neg c) == scalar_neg (inner_prod r c))
+      [SMTPat (inner_prod r (vec_neg c))] =
+  match r with
+  | Vec1 _ -> let Vec1 _ = c in ()
+  | VecN r' _ -> let VecN c' _ = c in inner_prod_neg_r r' c'
+
+let rec vec_scalar_mul_assoc (#o: orient) (#n: pos) (v: vec o n) (a1 a2: num)
+    : Lemma (vec_scalar_mul (vec_scalar_mul v a1) a2 == vec_scalar_mul v (scalar_mul a1 a2))
+      [SMTPat (vec_scalar_mul (vec_scalar_mul v a1) a2)] =
+  match v with
+  | Vec1 a -> scalar_mul_assoc a a1 a2
+  | VecN v' x ->
+    vec_scalar_mul_assoc v' a1 a2;
+    scalar_mul_assoc x a1 a2
+
+let rec vec_scalar_mul_add_dist (#o: orient) (#n: pos) (v1 v2: vec o n) (a: num)
+    : Lemma (vec_scalar_mul (vec_add v1 v2) a == vec_add (vec_scalar_mul v1 a) (vec_scalar_mul v2 a))
+      [SMTPat (vec_scalar_mul (vec_add v1 v2) a)] =
+  match v1 with
+  | Vec1 _ -> let Vec1 _ = v2 in ()
+  | VecN v1' _ -> let VecN v2' _ = v2 in vec_scalar_mul_add_dist v1' v2' a
+
+let rec inner_prod_scalar_r (#n: pos) (r: rvec n) (c: cvec n) (a: num)
+    : Lemma (inner_prod r (vec_scalar_mul c a) == scalar_mul (inner_prod r c) a)
+      [SMTPat (inner_prod r (vec_scalar_mul c a))] =
+  match r with
+  | Vec1 x ->
+    let Vec1 y = c in
+    scalar_mul_assoc x y a
+  | VecN r' rx ->
+    let VecN c' cy = c in
+    inner_prod_scalar_r r' c' a;
+    scalar_mul_assoc rx cy a
+    
