programs/LU.fst
@@ -7,8 +7,8 @@ let rec lu (#n:pos) (m:mat n{rowsdd m \/ spd m}) :
   u:mat n{upper u /\ nnz_diag u /\ mat_mul l u == m} =
   match m with
   | Mat1 a -> (|id_mat, m|)
-  | MatN d c a b ->
-    let s = schur1 d c a b in
+  | MatN m' c a b ->
+    let s = schur1 m in
     let (|l, u|) = lu s in
     let lc = vec_scalar_div c a in
     let l' = MatN l lc one zero_rvec in
