src/Scalar.fst
@@ -21,6 +21,9 @@ assume val scalar_mul (a1 a2: num) : a3: num
         (is_pos a1 /\ is_pos a2 ==> is_pos a3) /\ (is_nnz a1 /\ is_nnz a2 ==> is_nnz a3) /\
         (is_zero a1 \/ is_zero a2 ==> is_zero a3) }
 
+assume val scalar_mul_assoc (a b c: num)
+    : Lemma (scalar_mul (scalar_mul a b) c == scalar_mul a (scalar_mul b c))
+
 (* division *)
 assume val scalar_div (a1: num) (a2: num{is_nnz a2}) : a3: num{scalar_mul a3 a2 == a1}
 
@@ -33,6 +36,10 @@ assume val scalar_add (a1 a2: num) : a3: num
       { (is_zero a1 ==> a2 == a3) /\ (is_zero a2 ==> a1 == a3) /\
         (is_pos a1 /\ is_pos a2 ==> is_pos a3) }
 
+assume val scalar_mul_add_dist_r (a b c: num)
+    : Lemma (scalar_mul (scalar_add a b) c == scalar_add (scalar_mul a c) (scalar_mul b c))
+      [SMTPat (scalar_mul (scalar_add a b) c)]
+
 (* square root *)
 assume val sqrt (a1: num{is_nneg a1})
     : a2:num{(is_pos a1 ==> is_pos a2) /\ (is_zero a1 <==> is_zero a2) /\ scalar_mul a2 a2 == a1}
@@ -44,6 +51,14 @@ assume val scalar_neg (a: num) : b: num
 
 assume val scalar_neg_involutive (a: num)
     : Lemma (scalar_neg (scalar_neg a) == a) [SMTPat (scalar_neg (scalar_neg a))]
+
+assume val scalar_neg_add_dist (a b: num)
+    : Lemma (scalar_neg (scalar_add a b) == scalar_add (scalar_neg a) (scalar_neg b))
+      [SMTPat (scalar_neg (scalar_add a b))]
+
+assume val scalar_mul_neg (a b: num)
+    : Lemma (scalar_mul a (scalar_neg b) == scalar_neg (scalar_mul a b))
+      [SMTPat (scalar_mul a (scalar_neg b))]
 
 (* subtraction *)
 let scalar_sub (a1 a2: num) : num = scalar_add a1 (scalar_neg a2)
